utils/Zeta.FilterMap.fst
@@ -1,0 +1,55 @@
+module Zeta.FilterMap
+
+let rec indexed_filter_map (#a #b:_)
+  (fm: filter_map_param_t a b)
+  (s: seq a)
+  : Tot (seq b)
+    (decreases length s)
+  = let n = length s in
+    if n = 0
+    then empty #b
+    else
+      let s' = prefix s (n - 1) in
+      let ms' = indexed_filter_map fm s' in
+      if fm.f s
+      then append1 ms' (fm.m s)
+      else ms'
+
+let rec indexed_filter_map_map (#a #b:_)
+  (fm: filter_map_param_t a b)
+  (s: seq a)
+  (i: seq_index s {fsat fm s i})
+  : Tot(j: (seq_index (indexed_filter_map fm s)) {let fms = indexed_filter_map fm s in
+                                              index fms j == map fm s i})
+    (decreases (length s))
+  = let n = length s - 1 in
+    let s' = prefix s n in
+    let ms' = indexed_filter_map fm s' in
+    if i = n
+    then length ms'
+    else indexed_filter_map_map fm s' i
+
+let rec indexed_filter_map_invmap (#a #b:_)
+  (fm: filter_map_param_t a b)
+  (s: seq a)
+  (j: seq_index (indexed_filter_map fm s))
+  : Tot (i:(seq_index s){ fsat fm s i /\ indexed_filter_map_map fm s i = j })
+    (decreases (length s))
+  = let n = length s - 1 in
+    let s' = prefix s n in
+    let ms' = indexed_filter_map fm s' in
+    if j = length ms'
+    then n
+    else indexed_filter_map_invmap fm s' j
+
+let rec lemma_indexed_filter_map (#a #b:_)
+  (fm: filter_map_param_t a b)
+  (s: seq a)
+  (i: seq_index s {fsat fm s i})
+  : Lemma (ensures (let j = indexed_filter_map_map fm s i in
+                    i = indexed_filter_map_invmap fm s j))
+          (decreases (length s))
+  = let n = length s - 1 in
+    let s' = prefix s n in
+    if i = n then ()
+    else lemma_indexed_filter_map fm s' i
