utils/Zeta.FilterMap.fsti
@@ -1,0 +1,53 @@
+module Zeta.FilterMap
+
+open FStar.Seq
+open Zeta.SeqAux
+
+noeq
+type filter_map_param_t (a b:_) =
+  | FM: f: ((s:seq a{length s > 0}) -> bool) ->
+        m: ((s:seq a{length s > 0 /\ f s}) -> b) -> filter_map_param_t a b
+
+let fsat #a #b (fm: filter_map_param_t a b) (s: seq a) (i: seq_index s)
+  = fm.f (prefix s (i+1))
+
+let map #a #b (fm: filter_map_param_t a b) (s: seq a) (i: seq_index s{fsat fm s i})
+  = fm.m (prefix s (i+1))
+
+val indexed_filter_map (#a #b:_)
+  (fm: filter_map_param_t a b)
+  (s: seq a)
+  : seq b
+
+val indexed_filter_map_map (#a #b:_)
+  (fm: filter_map_param_t a b)
+  (s: seq a)
+  (i: seq_index s {fsat fm s i})
+  : j: (seq_index (indexed_filter_map fm s)) {let fms = indexed_filter_map fm s in
+                                              index fms j == map fm s i}
+
+val indexed_filter_map_invmap (#a #b:_)
+  (fm: filter_map_param_t a b)
+  (s: seq a)
+  (j: seq_index (indexed_filter_map fm s))
+  : i:(seq_index s){ fsat fm s i /\ indexed_filter_map_map fm s i = j }
+
+val lemma_indexed_filter_map (#a #b:_)
+  (fm: filter_map_param_t a b)
+  (s: seq a)
+  (i: seq_index s {fsat fm s i})
+  : Lemma (ensures (let j = indexed_filter_map_map fm s i in
+                    i = indexed_filter_map_invmap fm s j))
+          [SMTPat (indexed_filter_map_map fm s i)]
+
+let tailf #a (f: a -> bool) (s: seq a{length s > 0})
+  = f (telem s)
+
+let tailm #a #b (f: a -> bool) (m: (x:a{f x}) -> b) (s: seq a{length s > 0 /\ tailf f s})
+  = m (telem s)
+
+let tail_fmparam_t #a #b (f: a -> bool) (m: (x:a{f x}) -> b)
+  = FM (tailf f) (tailm f m)
+
+let simple_filter_map (#a #b:_) (f: a -> bool) (m: (x:a {f x}) -> b)
+  = indexed_filter_map (tail_fmparam_t f m)
